doc/coq/simple/Linking.v
@@ -1,158 +1,272 @@
-From Simple Require Export Abstract.
+From Simple Require Export Concrete.
 Require Export Coq.Logic.FunctionalExtensionality.
 
 Generalizable Variables T BT AT.
 
-Definition inject_ctx_mem `{Eq T} (Cout : @dy_ctx T) (mem : T -> list expr_value) :=
-  fun t => map (inject_ctx_v Cout) (mem t).
+Definition inject_ctx_mem `{Eq T} (Cout : @dy_ctx T) (mem : T -> option expr_value) :=
+  fun t => match mem t with None => None | Some v => Some (inject_ctx_v Cout v) end.
 
-Definition delete_ctx_mem `{Eq T} (Cout : @dy_ctx T) (mem : T -> list expr_value) :=
-  fun t => map (delete_ctx_v Cout) (mem t).
+Definition delete_ctx_mem `{Eq T} (Cout : @dy_ctx T) (mem : T -> option expr_value) :=
+  fun t => match mem t with None => None | Some v => Some (delete_ctx_v Cout v) end.
 
 Lemma delete_ctx_mem_eq :
-  forall `{Eq T} (Cout : @dy_ctx T) (mem : T -> list expr_value),
+  forall `{Eq T} (Cout : @dy_ctx T) (mem : T -> option expr_value),
          delete_ctx_mem Cout (inject_ctx_mem Cout mem) = mem.
 Proof.
   intros. apply functional_extensionality.
   intros. unfold inject_ctx_mem. unfold delete_ctx_mem.
-  remember (mem x) as l. clear Heql x mem. revert Cout.
-  induction l; try reflexivity. intros.
-  destruct a; simpl.
-  rewrite delete_inject_eq.
-  rewrite IHl. reflexivity.
+  destruct (mem x); eauto.
+  simpl. destruct e; simpl; rewrite delete_inject_eq.
+  eauto.
 Qed.
 
-Inductive link {BT AT} :=
-  | BF (t : BT)
-  | AF (t : AT)
+Inductive link `{Eq BT} `{Eq AT} :=
+  | L (bf : BT) (af : AT)
 .
 
-Definition link_eqb `{Eq BT} `{Eq AT} (t t' : @link BT AT) :=
-  match t, t' with
-  | BF t, BF t' => eqb t t'
-  | AF t, AF t' => eqb t t'
-  | _, _ => false
+Definition link_eqb `{EB : Eq BT} `{EA : Eq AT} 
+  (t1 : @link BT EB AT EA) (t2 : @link BT EB AT EA) :=
+  match t1, t2 with
+  | L bf af, L bf' af' =>
+    eqb bf bf' && eqb af af'
   end.
 
-Lemma link_eqb_eq `{Eq BT} `{Eq AT} :
-  forall (t t' : @link BT AT), link_eqb t t' = true <-> t = t'.
+Definition link_leb `{EB : Eq BT} `{@OrderT BT EB} `{EA : Eq AT} `{@OrderT AT EA} 
+  (t1 : @link BT EB AT EA) (t2 : @link BT EB AT EA) :=
+  match t1, t2 with
+  | L bf af, L bf' af' =>
+    if leb bf bf' then
+      if eqb bf bf' then
+        leb af af'
+      else true
+    else false
+  end.
+
+Lemma link_leb_refl : 
+  forall 
+    `{EB : Eq BT} `{EA : Eq AT}
+    `{OB : @OrderT BT EB} `{OA : @OrderT AT EA} t,
+  @link_leb BT EB OB AT EA OA t t = true.
+Proof.
+  intros. destruct t. simpl. rewrite leb_refl. 
+  replace (eqb bf bf) with true.
+  apply leb_refl.
+  symmetry. apply eqb_eq. eauto.
+Qed.
+
+Lemma link_leb_trans :
+  forall 
+    `{EB : Eq BT} `{EA : Eq AT}
+    `{OB : @OrderT BT EB} `{OA : @OrderT AT EA}
+    t t' t''
+    (LE : @link_leb BT EB OB AT EA OA t t' = true)
+    (LE' : @link_leb BT EB OB AT EA OA t' t'' = true),
+  link_leb t t'' = true.
 Proof.
   intros.
-  destruct t; destruct t'; simpl; split; intros EQ; 
-  try rewrite eqb_eq in *;
-  try inversion EQ;
-  subst; eauto.
+  destruct t as [bf af]; destruct t' as [bf' af'];
+  destruct t'' as [bf'' af'']; simpl in *.
+  destruct (leb bf bf') eqn:LEbf;
+  destruct (leb bf' bf'') eqn:LEbf';
+  try (inversion LE; fail);
+  try (inversion LE'; fail).
+  - destruct (eqb bf bf') eqn:EQbf;
+    destruct (eqb bf' bf'') eqn:EQbf';
+    try rewrite eqb_eq in *;
+    try rewrite eqb_neq in *;
+    replace (leb bf bf'') with true;
+    try (symmetry; apply leb_trans with (t' := bf'); eauto).
+    replace (eqb bf bf'') with true.
+    apply leb_trans with (t' := af'); eauto.
+    symmetry. apply eqb_eq; subst; eauto.
+    replace (eqb bf bf'') with false. eauto.
+    symmetry. apply eqb_neq. red. intros. subst.
+    apply EQbf'. eauto.
+    replace (eqb bf bf'') with false. eauto.
+    symmetry. apply eqb_neq. red. intros. subst.
+    apply EQbf. eauto.
+    replace (eqb bf bf'') with false. eauto.
+    symmetry. apply eqb_neq. red. intros. subst.
+    apply EQbf. apply leb_sym; eauto.
 Qed.
 
-Lemma link_eqb_neq `{Eq BT} `{Eq AT} :
-  forall (t t' : @link BT AT), link_eqb t t' = false <-> t <> t'.
+Lemma link_leb_sym :
+  forall 
+    `{EB : Eq BT} `{EA : Eq AT}
+    `{OB : @OrderT BT EB} `{OA : @OrderT AT EA} t t'
+    (LE : @link_leb BT EB OB AT EA OA t t' = true)
+    (LE' : @link_leb BT EB OB AT EA OA t' t = true),
+  t = t'.
 Proof.
-  intros. split; intros NEQ.
-  - red. intros contra. rewrite <- link_eqb_eq in contra.
-    rewrite NEQ in contra. inversion contra.
-  - refl_bool. intros contra. rewrite link_eqb_eq in contra.
-    apply NEQ. eauto.
+  intros.
+  destruct t as [bf af]; destruct t' as [bf' af'];
+  simpl in *;
+  destruct (leb bf bf') eqn:LEbf;
+  destruct (leb bf' bf) eqn:LEbf';
+  try (inversion LE; fail);
+  try (inversion LE'; fail).
+  assert (bf' = bf) as RR.
+  apply leb_sym; eauto.
+  rewrite RR in *.
+  replace (eqb bf bf) with true in *.
+  assert (af = af').
+  apply leb_sym; eauto. subst; eauto.
+  symmetry. apply eqb_eq. eauto.
 Qed.
 
-#[export] Instance link_eq `{Eq BT} `{Eq AT} : Eq (@link BT AT) :=
+Lemma link_eqb_eq :
+  forall `{EB : Eq BT} `{EA : Eq AT} t t',
+  @link_eqb BT EB AT EA t t' = true <-> t = t'.
+Proof.
+  intros.
+  destruct t as [bf af]; destruct t' as [bf' af'];
+  simpl in *;
+  split; intro EQ.
+  destruct (eqb bf bf') eqn:EQbf;
+  destruct (eqb af af') eqn:EQaf;
+  try (inversion EQ; fail).
+  rewrite eqb_eq in EQbf.
+  rewrite eqb_eq in EQaf. subst; eauto.
+  inversion EQ; subst.
+  replace (eqb bf' bf') with true;
+  try replace (eqb af' af') with true;
+  eauto; symmetry; apply eqb_eq; eauto.
+Qed.
+
+Lemma link_eqb_neq :
+  forall `{EB : Eq BT} `{EA : Eq AT} t t',
+  @link_eqb BT EB AT EA t t' = false <-> t <> t'.
+Proof.
+  intros.
+  split; intro NEQ.
+  red. intros EQ.
+  assert (link_eqb t t' = true) as RR. apply link_eqb_eq. eauto.
+  rewrite RR in NEQ. inversion NEQ.
+  refl_bool. intros contra. rewrite link_eqb_eq in contra.
+  apply NEQ; eauto.
+Qed.
+
+#[export] Instance LinkEq `{EB : Eq BT} `{EA : Eq AT} :
+  Eq (@link BT EB AT EA) :=
+{
+  eqb := link_eqb;
+  eqb_eq := link_eqb_eq;
+  eqb_neq := link_eqb_neq
+}.
+
+#[export] Instance LinkOrderT `{EB : Eq BT} `{EA : Eq AT} `{OB : @OrderT BT EB} `{OA : @OrderT AT EA} :
+  @OrderT (@link BT EB AT EA) LinkEq :=
   {
-    eqb := link_eqb;
-    eqb_eq := link_eqb_eq;
-    eqb_neq := link_eqb_neq
+    leb := link_leb;
+    leb_refl := link_leb_refl;
+    leb_trans := link_leb_trans;
+    leb_sym := link_leb_sym
   }.
 
-Fixpoint filter_ctx_bf {BT AT} (C : @dy_ctx (@link BT AT)) :=
+Fixpoint filter_ctx_bf
+  `{EB : Eq BT} `{EA : Eq AT}
+  (C : @dy_ctx (@link BT EB AT EA)) :=
   match C with
-  | [||] => [||]
+  | ([||]) => ([||])
   | dy_c_lam x t C' =>
     match t with
-    | BF t => dy_c_lam x t (filter_ctx_bf C')
-    | AF t => filter_ctx_bf C'
+    | L bf af => dy_c_lam x bf (filter_ctx_bf C')
     end
   | dy_c_lete x t C' =>
     match t with
-    | BF t => dy_c_lete x t (filter_ctx_bf C')
-    | AF t => filter_ctx_bf C'
+    | L bf af => dy_c_lete x bf (filter_ctx_bf C')
     end
-  | dy_c_letm M C' C'' => dy_c_letm M (filter_ctx_bf C') (filter_ctx_bf C'')
+  | dy_c_letm M C' C'' =>
+    dy_c_letm M (filter_ctx_bf C') (filter_ctx_bf C'')
   end.
 
-Fixpoint filter_ctx_af {BT AT} (C : @dy_ctx (@link BT AT)) :=
+Fixpoint filter_ctx_af
+  `{EB : Eq BT} `{EA : Eq AT}
+  (C : @dy_ctx (@link BT EB AT EA)) :=
   match C with
-  | [||] => [||]
+  | ([||]) => ([||])
   | dy_c_lam x t C' =>
     match t with
-    | AF t => dy_c_lam x t (filter_ctx_af C')
-    | BF t => filter_ctx_af C'
+    | L bf af => dy_c_lam x af (filter_ctx_af C')
     end
   | dy_c_lete x t C' =>
     match t with
-    | AF t => dy_c_lete x t (filter_ctx_af C')
-    | BF t => filter_ctx_af C'
+    | L bf af => dy_c_lete x af (filter_ctx_af C')
     end
-  | dy_c_letm M C' C'' => dy_c_letm M (filter_ctx_af C') (filter_ctx_af C'')
+  | dy_c_letm M C' C'' =>
+    dy_c_letm M (filter_ctx_af C') (filter_ctx_af C'')
   end.
 
-Definition filter_v_bf {BT AT} (v : @expr_value (@link BT AT)) :=
+Definition filter_mem_bf
+  `{EB : Eq BT} `{EA : Eq AT} (init : AT)
+  (mem : (@link BT EB AT EA) -> option (@expr_value (@link BT EB AT EA))) :=
+  fun t =>
+    match mem (L t init) with
+    | Some (Closure x e C) => Some (Closure x e (filter_ctx_bf C))
+    | None => None
+    end.
+
+Definition filter_mem_af
+  `{EB : Eq BT} `{EA : Eq AT} (final : BT)
+  (mem : (@link BT EB AT EA) -> option (@expr_value (@link BT EB AT EA))) :=
+  fun t =>
+    match mem (L final t) with
+    | Some (Closure x e C) => Some (Closure x e (filter_ctx_af C))
+    | None => None
+    end.
+
+Definition filter_v_bf 
+  `{EB : Eq BT} `{EA : Eq AT}
+  (v : @expr_value (@link BT EB AT EA)) :=
   match v with
   | Closure x e C => Closure x e (filter_ctx_bf C)
   end.
 
-Definition filter_v_af {BT AT} (v : @expr_value (@link BT AT)) :=
+Definition filter_v_af
+  `{EB : Eq BT} `{EA : Eq AT}
+  (v : @expr_value (@link BT EB AT EA)) :=
   match v with
   | Closure x e C => Closure x e (filter_ctx_af C)
   end.
 
-Definition filter_mem_bf {BT AT} (mem : (@link BT AT) -> list (@expr_value (@link BT AT))) :=
-  fun t => map filter_v_bf (mem (BF t))
-.
-
-Definition filter_mem_af {BT AT} (mem : (@link BT AT) -> list (@expr_value (@link BT AT))) :=
-  fun t => map filter_v_af (mem (AF t))
-.
-
-Fixpoint lift_ctx_bf {BT AT} C : @dy_ctx (@link BT AT) :=
+Fixpoint lift_ctx_bf `{EB : Eq BT} `{EA : Eq AT} (init : AT) (C : @dy_ctx BT)
+  : @dy_ctx (@link BT EB AT EA) :=
   match C with
-  | [||] => [||]
-  | dy_c_lam x t C' => dy_c_lam x (BF t) (lift_ctx_bf C')
-  | dy_c_lete x t C' => dy_c_lete x (BF t) (lift_ctx_bf C')
-  | dy_c_letm M C' C'' => dy_c_letm M (lift_ctx_bf C') (lift_ctx_bf C'')
+  | ([||]) => ([||])
+  | dy_c_lam x t C' => dy_c_lam x (L t init) (lift_ctx_bf init C')
+  | dy_c_lete x t C' => dy_c_lete x (L t init) (lift_ctx_bf init C')
+  | dy_c_letm M C' C'' => dy_c_letm M (lift_ctx_bf init C') (lift_ctx_bf init C'')
   end.
 
-Definition lift_v_bf {BT AT} v : @expr_value (@link BT AT) :=
-  match v with
-  | Closure x e C => Closure x e (lift_ctx_bf C)
-  end.
-
-Fixpoint lift_ctx_af {BT AT} C : @dy_ctx (@link BT AT) :=
+Fixpoint lift_ctx_af `{EB : Eq BT} `{EA : Eq AT} (final : BT) (C : @dy_ctx AT)
+  : @dy_ctx (@link BT EB AT EA) :=
   match C with
-  | [||] => [||]
-  | dy_c_lam x t C' => dy_c_lam x (AF t) (lift_ctx_af C')
-  | dy_c_lete x t C' => dy_c_lete x (AF t) (lift_ctx_af C')
-  | dy_c_letm M C' C'' => dy_c_letm M (lift_ctx_af C') (lift_ctx_af C'')
+  | ([||]) => ([||])
+  | dy_c_lam x t C' => dy_c_lam x (L final t) (lift_ctx_af final C')
+  | dy_c_lete x t C' => dy_c_lete x (L final t) (lift_ctx_af final C')
+  | dy_c_letm M C' C'' => dy_c_letm M (lift_ctx_af final C') (lift_ctx_af final C'')
   end.
 
-Definition lift_v_af {BT AT} v : @expr_value (@link BT AT) :=
-  match v with
-  | Closure x e C => Closure x e (lift_ctx_af C)
-  end.
+(*
+Definition link_tick `{time BT} `{time AT} (final : BT) (init : AT) (Cout : @dy_ctx BT)
+  C st x v :=
+  match st with
+  | ST mem t =>
+    match t with
+    | L bt t =>
+      if leb final bt then
+        L bt (tick )
+      else if 
 
-Definition link_tick `{time BT} `{time AT} (Cout : @dy_ctx BT) :=
-  fun C st x v =>
-    match st with
-    | ST mem t =>
-      match t with
-      | BF t => BF (tick (filter_ctx_bf C) (ST (filter_mem_bf mem) t) x (filter_v_bf v))
-      | AF t =>
         let Cout := lift_ctx_bf Cout in
         AF
         (tick (filter_ctx_af (delete_ctx Cout C))
                 (ST (filter_mem_af (delete_ctx_mem Cout mem)) t)
                 x (filter_v_af (delete_ctx_v Cout v)))
       end
-    end.
+  end.
 
-#[export] Instance link_time `{time BT} `{time AT} (Cout : @dy_ctx BT) : (@time (@link BT AT) (@link_eq BT _ AT _)) :=
+#[export] Instance link_time `{Eq BT} `{time AT} (Cout : @dy_ctx BT) : (@time (@link BT AT) (@link_eq BT _ AT _)) :=
   {
     tick := link_tick Cout
   }.
@@ -198,7 +312,7 @@ Proof.
   rewrite delete_inject_eq. rewrite filter_lift_eq_af. eauto.
 Qed.
 
-Lemma link_tick_eq `{time BT} `{time AT} (Cout : @dy_ctx BT) :
+Lemma link_tick_eq `{Eq BT} `{time AT} (Cout : @dy_ctx BT) :
   forall bmem C amem t x v,
     link_tick Cout ((lift_ctx_bf Cout)<|(lift_ctx_af C)|>)
                 (ST (link_mem bmem Cout amem) (AF t)) x 
@@ -213,7 +327,7 @@ Proof.
   reflexivity.
 Qed.
 
-Lemma link_update_m_eq `{time BT} `{time AT} (Cout : @dy_ctx BT):
+Lemma link_update_m_eq `{Eq BT} `{time AT} (Cout : @dy_ctx BT):
   forall bmem amem t v,
   (AF t !#-> inject_ctx_v (lift_ctx_bf Cout) (lift_v_af v);
     (link_mem bmem Cout amem)) =
@@ -261,7 +375,7 @@ Proof.
   rewrite IHC2. eauto.
 Qed.
 
-Lemma link_eval_eq `{time BT} `{time AT} (Cout : @dy_ctx BT) :
+Lemma link_eval_eq `{Eq BT} `{time AT} (Cout : @dy_ctx BT) :
   forall bmem C st e v st'
          (EVAL : @EvalR AT _ _ C st e v st'),
     let inject_C := (lift_ctx_bf Cout) <|(lift_ctx_af C)|> in
@@ -327,7 +441,7 @@ Proof.
     rewrite RR. clear RR. simpl in *. exact IHEVAL2.
 Qed.
 
-Lemma link_reach_eq `{time BT} `{time AT} (Cout : @dy_ctx BT) :
+Lemma link_reach_eq `{Eq BT} `{time AT} (Cout : @dy_ctx BT) :
   forall bmem C st e C' st' e'
          (REACH : @one_reach AT _ _ C st e C' st' e'),
     let inject_C := (lift_ctx_bf Cout) <|(lift_ctx_af C)|> in
@@ -393,3 +507,4 @@ Proof.
     simpl in *.
     eapply one_letmr; simpl in *; eauto.
 Qed.
+*)
